1(a)

(i)
```
[7, 5, 4]
Node(Node(Leaf 7)(Leaf 5))(Node (Leaf 4))
[4, 5, 7]
```

(ii)
Principle of structural induction (for *trees*):    
$[\forall x:a. \texttt{P(Leaf}x\texttt{)} \wedge 
\forall t1, t2: \texttt{Tree a}.  P(t1) \wedge P(t2) \rightarrow \texttt{P(Node(t1 t2))}]$
$\rightarrow \forall t : \texttt{Tree a}.P(t)$     

(iii)
What is to be shown:    
*Base case*: $\forall x:a . rev(fringe (Leaf x)) = fringe(mirror (Leaf x))$    
*Inductive case*: We assume $\forall t1, t2:Tree a$    
rev(fringe(t1)) = fringe(mirror(t1)) *and*    
rev(fringe(t2)) = fringe(mirror(t2))    
and then show that:
$\forall x:a$. rev(fringe(Node (t1 a t2))) = fringe(mirror(Node (t1 a t2)))

1.(b) 

(i) 
Proof using *multiple induction*.    
Outer proof uses structural induction (for *trees*) on ts    
Inner proof uses structural induction (for *lists*) on t
- Base Case:    
To show: frngTR((Leaf x):ts) xs = frngTR ts (xs++(fringe (Leaf x)))    
LHS = frngTR ts (xs++[x])    
RHS = frngTR ts (xs++[x])    
We have LHS = RHS, so base case holds.

- Inductive case.    
For all ts, xs, assume P(t1, ts) and P(t2, ts)    
to show P(Node(t1, t2), ts)
    - Base case.     
    To show: P(Node(t1, t2), [])    
    frngTR (Node(t1, t2):[]) xs = frngTR [] (xs++(fringe (Node(t1, t2))))
    LHS = frngTR(t1:t2) xs     
        = frngTR t2 (xs++(fringe t1)) (by induction hypothesis, P(t1, ts))    
        = frngTR [] xs++(fringe t1)++(fringe t2) (by induction hypothesis, P(t2, ts))    
        = xs++(fringe t1)++(fringe t2)   
    RHS = xs++(fringe Node(t1, t2))    
        = xs++(fringe t1) ++ (fringe t2)    
    - Inductive case:     
    Assume P(Node(t1, t2), ts)    
    To show: P(Node(t1, t2), (t:ts))    
    frngTR(Node(t1, t2):(t:ts)) xs = frngTR (t:ts) (xs++(fringe (Node(t1, t2))))
        - case: t = Leaf y    
        LHS = frngTR (t1:t2:(Leaf y):ts) xs    
            = frngTR (t2:(Leaf y):ts) (xs++(fringe t1))    
            = frngTR ((Leaf y):ts) (xs++(fringet1)++(fringe t2))    
            = frngTR ts (xs++(fringet1)++(fringe t2)++[y])    
        RHS = frngTR ((Leaf y):ts) (xs++(fringe t1)++(fringe t2))    
            = frngTR ts (xs++(fringet1)++(fringe t2)++[y])    
        - case: t = (Node x y)    
        ```
        LHS = frngTR (t1:t2:(Node x y):ts) xs    
            = frngTR (t2:(Node x y):ts) (xs++(fringe t1))    
            = frngTR ((Node x y):ts) (xs++(fringet1)++(fringe t2))    
        RHS = frngTR ((Node x y):ts) (xs++(fringe t1)++(fringe t2))    
        ```
    
    - In both cases LHS=RHS, so inner inductive case holds.
    - Both inner base and inner inductive cases hold.    
      Hence P(Node(t1, t2), ts) holds.

Both outer base and outer inductive hold.    
Hence P(t, ts) holds.

(ii)
Structural induction (for *trees*) on t.    
- Base case:
  ```
  fringe (Leaf z) = frngTR [Leaf z] []
  ```
  LHS = [z]
  RHS = frngTR [] [fringe (Leaf z)]
      = frngTR [] [z]
      = [z]
  Hence base case holds.
- Inductive case:
  ```
  fringe (Node t1 t2) = frngTR [(Node t1 t2)] []
  ```
  LHS = (fringe t1)++(fringe t2)
  RHS = frngTR (t1:t2) []
      = frngTR [t2] ([]++fringe(t1))
      = frngTR [] ([]++(fringe t1)++(fringe t2))
      = []++(fringe t1)++(fringe t2))
      = (fringe t1)++(fringe t2)
- So by induction, property holds for all t.



2.

(a) $swap(a, b, i, j) \Leftrightarrow a.length = b.length$    
$\wedge i, j \in [0..a.length]$    
$\wedge b[i] = a[j]$    
$\wedge b[j] = a[i]$    
$k \in [0..a.length] - \{i, j\} \Rightarrow b[k] = a[k]$   

(b) Invariant:    
Perm(a, a0)

(c)     
Let a1 denote a before kth iteration
Let a2 denote a after kth iteration.
Given: Perm(a1, a0)
To show: Perm(a2, a0)
Proof:
We have `swap(a1, i-1, r)` that gives $swap(a2, a1, i-1, r)$.
From lemma 1, this gives $Perm(a2, a1)$.
But Perm(a1, a0). So Perm(a2, a0).

(d) `a = ['b', 'c', 'd', 'e', 'a']`




